src/Rupicola/Examples/Loops.v
@@ -16,12 +16,6 @@ Section Ex.
 
   Open Scope Z_scope.
 
-  Notation "∅" := map.empty.
-  Notation "m [[ k ← v ]]" :=
-    (map.put m k v)
-      (left associativity, at level 1,
-       format "m [[ k  ←  v ]]").
-
   Lemma signed_lt_unsigned (w : word):
     word.signed w <= word.unsigned w.
   Proof.
@@ -38,13 +32,12 @@ Section Ex.
           (a2: VectorArray.t word n2)
           (pr1: word.unsigned len < Z.of_nat n1)
           (pr2: word.unsigned len < Z.of_nat n2) :=
-    let/n from := word.of_Z 0 in
-    let/n (from, a2) := ranged_for_u
-                         from len
-                         (fun a2 tok idx Hlt =>
-                            let/n v := VectorArray.get a1 idx _ in
-                            let/n a2 := VectorArray.put a2 idx _ v in
-                            (tok, a2)) a2 in
+    let/n a2 := ranged_for_u
+                 (word.of_Z 0) len
+                 (fun a2 tok idx Hlt =>
+                    let/n v := VectorArray.get a1 idx _ in
+                    let/n a2 := VectorArray.put a2 idx _ v in
+                    (tok, a2)) a2 in
     (a1, a2).
   Next Obligation.
     pose proof word.unsigned_range idx.
@@ -88,24 +81,23 @@ Section Ex.
           (a2: VectorArray.t word n2)
           (pr1: word.signed len < Z.of_nat n1)
           (pr2: word.signed len < Z.of_nat n2) :=
-    let/n from eq:_ := word.of_Z 0 in
-    let/n (from, a2) := ranged_for_s
-                         from len
-                         (fun a2 tok idx Hlt =>
-                            let/n v := VectorArray.get a1 idx _ in
-                            let/n a2 := VectorArray.put a2 idx _ v in
-                            (tok, a2)) a2 in
+    let/n a2 := ranged_for_s
+                 (word.of_Z 0) len
+                 (fun a2 tok idx Hlt =>
+                    let/n v := VectorArray.get a1 idx _ in
+                    let/n a2 := VectorArray.put a2 idx _ v in
+                    (tok, a2)) a2 in
     (a1, a2).
   Next Obligation.
     pose proof word.half_modulus_pos (word:=word).
     unfold cast, Convertible_word_nat.
-    rewrite word.signed_of_Z, word.swrap_inrange in H0 by lia.
+    rewrite word.signed_of_Z, word.swrap_inrange in H by lia.
     rewrite word.signed_gz_eq_unsigned; lia.
   Qed.
   Next Obligation.
     pose proof word.half_modulus_pos (word:=word).
     unfold cast, Convertible_word_nat.
-    rewrite word.signed_of_Z, word.swrap_inrange in H0 by lia.
+    rewrite word.signed_of_Z, word.swrap_inrange in H by lia.
     rewrite word.signed_gz_eq_unsigned; lia.
   Qed.
 
@@ -136,13 +128,12 @@ Section Ex.
   Definition list_memcpy (len: word)
              (a1: ListArray.t word)
              (a2: ListArray.t word) :=
-    let/n from := word.of_Z 0 in
-    let/n (from, a2) := ranged_for_u
-                         from len
-                         (fun a2 tok idx Hlt =>
-                            let/n v := ListArray.get a1 idx in
-                            let/n a2 := ListArray.put a2 idx v in
-                            (tok, a2)) a2 in
+    let/n a2 := ranged_for_u
+                 (word.of_Z 0) len
+                 (fun a2 tok idx Hlt =>
+                    let/n v := ListArray.get a1 idx in
+                    let/n a2 := ListArray.put a2 idx v in
+                    (tok, a2)) a2 in
     (a1, a2).
 
   Instance spec_of_sizedlist_memcpy : spec_of "sizedlist_memcpy" :=
@@ -197,7 +188,7 @@ Section Ex.
             implements list_memcpy)
            As unsizedlist_memcpy_correct.
     Proof.
-      compile.
+      compile_setup; repeat compile_step.
 
       { lia. (* loop index in bounds + function precondition *) }
       { (* Note the call to induction.
@@ -216,18 +207,15 @@ Section Ex.
   End Unsz.
 
   Program Definition incr_gallina (c: cell) : cell :=
-    let/n one := word.of_Z 1 in
-    let/n from := word.of_Z 3 in
-    let/n to := word.of_Z 5 in
     let/n tick := word.of_Z 0 in
-    let/n (from, tick, c) :=
+    let/n (tick, c) :=
        ranged_for_u
-         from to
+         (word.of_Z 3) (word.of_Z 5)
          (fun '\< tick, c \> tok idx bounded =>
             let/n v := get c in
             let/n v := word.add v idx in
             let/n c := put v in
-            let/n tick := word.add tick one in
+            let/n tick := word.add tick (word.of_Z 1) in
             (tok, \< tick, c \>))
          \< tick, c \> in
     (let/n v := get c in
